theories/F_mu_ref/unary/soundness.v
@@ -1,15 +1,17 @@
 From WBLogrel.F_mu_ref.unary Require Export fundamental.
+From iris.algebra Require Import auth.
 From iris.proofmode Require Import proofmode.
 From iris.program_logic Require Import adequacy.
 From iris.prelude Require Import options.
 
-Class heapPreIG Σ := HeapPreIG {
-  heap_preG_iris :> invGpreS Σ;
-  heap_preG_heap :> gen_heapGpreS loc F_mu_ref.val Σ
+Class soundness_unary_preG Σ := soundness_unary_preIG {
+  soundness_unary_preG_iris :> invGpreS Σ;
+  soundness_unary_preG_heap :> gen_heapGpreS loc F_mu_ref.val Σ;
+  soundness_unary_preG_reg :> inG Σ (authUR ghost_regUR)
 }.
 
-Theorem soundness Σ `{heapPreIG Σ} e τ e' thp σ σ' :
-  (∀ `{heapIG Σ}, ⊢ [] ⊨ e : τ) →
+Theorem soundness Σ `{soundness_unary_preG Σ} e τ e' thp σ σ' :
+  (∀ `{heapIG Σ, ghost_regG Σ}, ⊢ [] ⊨ e : τ) →
   rtc erased_step ([e], σ) (thp, σ') → e' ∈ thp →
   not_stuck e' σ'.
 Proof.
@@ -20,9 +22,10 @@ Proof.
   iMod (gen_heap_init σ) as (Hheap) "[Hh _]".
   iModIntro. iExists (λ σ _, gen_heap_interp σ), (λ _, True%I); iFrame.
   set (HeapΣ := (HeapIG Σ Hinv Hheap)).
-  iApply (wp_wand with "[]").
+  iMod ghost_reg_init as (?) "Hreg".
+  iApply (wp_wand with "[Hreg]").
   - replace e with e.[env_subst[]] by by asimpl.
-    iApply (Hlog HeapΣ $! [] []). iApply (@interp_env_nil _ HeapΣ).
+    iApply (Hlog HeapΣ $! [] []); [iApply (@interp_env_nil _ HeapΣ)|iFrame].
   - eauto.
 Qed.
 
@@ -30,7 +33,7 @@ Corollary type_soundness e τ e' thp σ σ' :
   [] ⊢ₜ e : τ →
   rtc erased_step ([e], σ) (thp, σ') → e' ∈ thp → not_stuck e' σ'.
 Proof.
-  intros ??. set (Σ := #[invΣ ; gen_heapΣ loc F_mu_ref.val]).
-  set (HG := HeapPreIG Σ _ _).
+  intros ??. set (Σ := #[invΣ ; gen_heapΣ loc F_mu_ref.val; ghost_regΣ]).
+  set (HG := soundness_unary_preIG Σ _ _ _).
   eapply (soundness Σ); eauto using fundamental.
 Qed.
