theories/F_mu_ref/binary/fundamental.v
@@ -5,7 +5,7 @@ From WBLogrel.F_mu_ref.binary Require Export logrel rules.
 From iris.prelude Require Import options.
 
 Section bin_log_def.
-  Context `{heapIG Σ, cfgSG Σ}.
+  Context `{heapIG Σ, cfgSG Σ, ghost_regG Σ}.
   Notation D := (persistent_predO (val * val) (iPropI Σ)).
 
   Definition bin_log_related (Γ : list type) (e e' : expr) (τ : type) : iProp Σ :=
@@ -22,56 +22,77 @@ Notation "Γ ⊨ e '≤log≤' e' : τ" :=
   (bin_log_related Γ e e' τ) (at level 74, e, e', τ at next level).
 
 Section fundamental.
-  Context `{heapIG Σ, cfgSG Σ}.
+  Context `{heapIG Σ, cfgSG Σ, ghost_regG Σ}.
   Notation D := (persistent_predO (val * val) (iPropI Σ)).
   Implicit Types e : expr.
   Implicit Types Δ : listO D.
+  Implicit Type τi : listO D -n> D.
   Local Hint Resolve to_of_val : core.
 
-  Local Tactic Notation "smart_wp_bind" uconstr(ctx) ident(v) ident(w)
-        constr(Hv) uconstr(Hp) :=
-    iApply (wp_bind (fill [ctx]));
-    iApply (wp_wand with "[-]");
-      [iApply Hp; iFrame "#"; trivial|];
-    iIntros (v); iDestruct 1 as (w) Hv; simpl.
+  Lemma bin_expr_rel_bind K K' τi1 τi2 Δ e e' :
+    interp_expr τi1 Δ (e, e') -∗
+    (∀ v v', τi1 Δ (v, v') -∗ interp_expr τi2 Δ (fill K (of_val v), fill K' (of_val v'))) -∗
+    interp_expr τi2 Δ (fill K e, fill K' e').
+  Proof.
+    iIntros "Hee Hkk".
+    iIntros (M j Krs) "Hreg Hj /=".
+    iApply (wp_bind (fill K)).
+    rewrite -fill_app.
+    iApply (wp_wand with "[- Hkk]"); first by iApply ("Hee" with "Hreg Hj").
+    iIntros (v); simpl.
+    iDestruct 1 as (v' N1) "[Hreg [Hj #Hvv]]".
+    rewrite fill_app.
+    iApply ("Hkk" with "[$] [$] [$]").
+  Qed.
+
+  Lemma bin_val_rel_bin_expr_rel v v' τi Δ :
+    τi Δ (v, v') -∗ interp_expr τi Δ (of_val v, of_val v').
+  Proof.
+    iIntros "#?".
+    iIntros (M j Krs) "Hreg Hj /=".
+    iApply wp_value.
+    iExists _, _; iFrame; done.
+  Qed.
 
   (* Put all quantifiers at the outer level *)
-  Lemma bin_log_related_alt {Γ e e' τ} Δ vvs j K :
+  Lemma bin_log_related_alt {Γ e e' τ} Δ vvs M j K :
     Γ ⊨ e ≤log≤ e' : τ -∗
-    spec_ctx ∗ ⟦ Γ ⟧* Δ vvs ∗ j ⤇ fill K (e'.[env_subst (vvs.*2)])
-    -∗ WP e.[env_subst (vvs.*1)] {{ v, ∃ v',
-        j ⤇ fill K (of_val v') ∗ interp τ Δ (v, v') }}.
+    spec_ctx ∗ ⟦ Γ ⟧* Δ vvs ∗ ghost_reg_full M ∗ j ⤇ fill K (e'.[env_subst (vvs.*2)])
+    -∗ WP e.[env_subst (vvs.*1)] {{ v, ∃ v' M',
+        ghost_reg_full M' ∗ j ⤇ fill K (of_val v') ∗ interp τ Δ (v, v') }}.
   Proof.
-    iIntros "#Hlog (#Hs & HΓ & Hj)".
-    iApply ("Hlog" with "[HΓ]"); iFrame; eauto.
+    iIntros "#Hee (#Hspec & #HΓ & Hreg & Hj)".
+    iSpecialize ("Hee" $! Δ vvs with "[$]").
+    iApply (wp_wand with "[-]"); first by iApply ("Hee" with "Hreg Hj").
+    iIntros (v) "?"; done.
   Qed.
 
   Lemma bin_log_related_var Γ x τ :
     Γ !! x = Some τ → ⊢ Γ ⊨ Var x ≤log≤ Var x : τ.
   Proof.
-    iIntros (? Δ vvs) "!# #(Hs & HΓ)"; iIntros (j K) "Hj /=".
+    iIntros (? Δ vvs) "!# #(Hs & HΓ)". iIntros (M j K) "Hreg Hj /=".
     iDestruct (interp_env_Some_l with "HΓ") as ([v v']) "[Heq ?]"; first done.
     iDestruct "Heq" as %Heq.
     erewrite !env_subst_lookup; rewrite ?list_lookup_fmap ?Heq; eauto.
-    iApply wp_value; eauto.
+    iApply wp_value; iExists _, _; iFrame; done.
   Qed.
 
   Lemma bin_log_related_unit Γ : ⊢ Γ ⊨ Unit ≤log≤ Unit : TUnit.
   Proof.
-    iIntros (Δ vvs) "!# #(Hs & HΓ)"; iIntros (j K) "Hj /=".
-    iApply wp_value. iExists UnitV; eauto.
+    iIntros (Δ vvs) "!# #(Hs & HΓ)"; iIntros (M j K) "Hreg Hj /=".
+    iApply wp_value. iExists UnitV, _; iFrame; eauto.
   Qed.
 
   Lemma bin_log_related_nat Γ n : ⊢ Γ ⊨ #n n ≤log≤ #n n : TNat.
   Proof.
-    iIntros (Δ vvs) "!# #(Hs & HΓ)"; iIntros (j K) "Hj /=".
-    iApply wp_value. iExists (#nv _); eauto.
+    iIntros (Δ vvs) "!# #(Hs & HΓ)"; iIntros (M j K) "Hreg Hj /=".
+    iApply wp_value. iExists (#nv _), _; iFrame; eauto.
   Qed.
 
   Lemma bin_log_related_bool Γ b : ⊢ Γ ⊨ #♭ b ≤log≤ #♭ b : TBool.
   Proof.
-    iIntros (Δ vvs) "!# #(Hs & HΓ)"; iIntros (j K) "Hj /=".
-    iApply wp_value. iExists (#♭v _); eauto.
+    iIntros (Δ vvs) "!# #(Hs & HΓ)"; iIntros (M j K) "Hreg Hj /=".
+    iApply wp_value. iExists (#♭v _), _; iFrame; eauto.
   Qed.
 
   Lemma bin_log_related_pair Γ e1 e2 e1' e2' τ1 τ2 :
@@ -79,57 +100,59 @@ Section fundamental.
     Γ ⊨ e2 ≤log≤ e2' : τ2 -∗
     Γ ⊨ Pair e1 e2 ≤log≤ Pair e1' e2' : TProd τ1 τ2.
   Proof.
-    iIntros "#IH1 #IH2" (Δ vvs) "!# #(Hs & HΓ)". iIntros (j K) "Hj /=".
-    smart_wp_bind (PairLCtx e2.[env_subst _]) v v' "[Hv #Hiv]"
-      (bin_log_related_alt _ _ j ((PairLCtx e2'.[env_subst _]) :: K) with "IH1").
-    smart_wp_bind (PairRCtx v) w w' "[Hw #Hiw]"
-      (bin_log_related_alt _ _ j ((PairRCtx v') :: K) with "IH2").
-    iApply wp_value. iExists (PairV v' w'); iFrame "Hw".
-    iExists (v, v'), (w, w'); simpl; repeat iSplit; trivial.
+    iIntros "#IH1 #IH2" (Δ vvs) "!# #(Hs & HΓ)".
+    iApply (bin_expr_rel_bind [PairLCtx _] [PairLCtx _]); first by iApply "IH1"; iFrame "#".
+    iIntros (v v') "Hvv /=".
+    iApply (bin_expr_rel_bind [PairRCtx _] [PairRCtx _]); first by iApply "IH2"; iFrame "#".
+    iIntros (w w') "Hww /=".
+    iApply (bin_val_rel_bin_expr_rel (PairV _ _) (PairV _ _)); simpl.
+    iExists _, _; repeat iSplit; eauto; simpl; done.
   Qed.
 
   Lemma bin_log_related_fst Γ e e' τ1 τ2 :
     Γ ⊨ e ≤log≤ e' : TProd τ1 τ2 -∗ Γ ⊨ Fst e ≤log≤ Fst e' : τ1.
   Proof.
-    iIntros "#IH" (Δ vvs) "!# #(Hs & HΓ)"; iIntros (j K) "Hj /=".
-    smart_wp_bind (FstCtx) v v' "[Hv #Hiv]"
-      (bin_log_related_alt _ _ j (FstCtx :: K) with "[IH]"); cbn.
-    iDestruct "Hiv" as ([w1 w1'] [w2 w2']) "#[% [Hw1 Hw2]]"; simplify_eq.
+    iIntros "#IH" (Δ vvs) "!# #(Hs & HΓ)".
+    iApply (bin_expr_rel_bind [FstCtx] [FstCtx]); first by iApply "IH"; iFrame "#".
+    iIntros (v v') "Hvv /=".
+    iDestruct "Hvv" as ([w1 w1'] [w2 w2']) "#[% [Hw1 Hw2]]"; simplify_eq/=.
+    iIntros (M j K) "Hreg Hj /=".
     iApply wp_pure_step_later; eauto. iNext.
-    iMod (step_fst with "[Hs Hv]") as "Hw"; eauto.
-    iApply wp_value; eauto.
+    iMod (step_fst with "[$]") as "Hw"; eauto.
+    iApply wp_value. iExists _, _; iFrame; done.
   Qed.
 
   Lemma bin_log_related_snd Γ e e' τ1 τ2 :
     Γ ⊨ e ≤log≤ e' : TProd τ1 τ2 -∗ Γ ⊨ Snd e ≤log≤ Snd e' : τ2.
   Proof.
-    iIntros "#IH" (Δ vvs) "!# #(Hs & HΓ)"; iIntros (j K) "Hj /=".
-    smart_wp_bind (SndCtx) v v' "[Hv #Hiv]"
-      (bin_log_related_alt _ _ j (SndCtx :: K) with "IH"); cbn.
-    iDestruct "Hiv" as ([w1 w1'] [w2 w2']) "#[% [Hw1 Hw2]]"; simplify_eq.
+    iIntros "#IH" (Δ vvs) "!# #(Hs & HΓ)".
+    iApply (bin_expr_rel_bind [SndCtx] [SndCtx]); first by iApply "IH"; iFrame "#".
+    iIntros (v v') "Hvv /=".
+    iDestruct "Hvv" as ([w1 w1'] [w2 w2']) "#[% [Hw1 Hw2]]"; simplify_eq/=.
+    iIntros (M j K) "Hreg Hj /=".
     iApply wp_pure_step_later; eauto. iNext.
-    iMod (step_snd with "[Hs Hv]") as "Hw"; eauto.
-    iApply wp_value; eauto.
+    iMod (step_snd with "[$]") as "Hw"; eauto.
+    iApply wp_value. iExists _, _; iFrame; done.
   Qed.
 
   Lemma bin_log_related_injl Γ e e' τ1 τ2 :
     Γ ⊨ e ≤log≤ e' : τ1 -∗ Γ ⊨ InjL e ≤log≤ InjL e' : (TSum τ1 τ2).
   Proof.
-    iIntros "#IH" (Δ vvs) "!# #(Hs & HΓ)"; iIntros (j K) "Hj /=".
-    smart_wp_bind (InjLCtx) v v' "[Hv #Hiv]"
-      (bin_log_related_alt _ _ j (InjLCtx :: K) with "IH"); cbn.
-    iApply wp_value. iExists (InjLV v'); iFrame "Hv".
-    iLeft; iExists (_,_); eauto 10.
+    iIntros "#IH" (Δ vvs) "!# #(Hs & HΓ)".
+    iApply (bin_expr_rel_bind [InjLCtx] [InjLCtx]); first by iApply "IH"; iFrame "#".
+    iIntros (v v') "Hvv /=".
+    iApply (bin_val_rel_bin_expr_rel (InjLV _) (InjLV _)).
+    iLeft; iExists (_, _); simpl; eauto.
   Qed.
 
   Lemma bin_log_related_injr Γ e e' τ1 τ2 :
       Γ ⊨ e ≤log≤ e' : τ2 -∗ Γ ⊨ InjR e ≤log≤ InjR e' : TSum τ1 τ2.
   Proof.
-    iIntros "#IH" (Δ vvs) "!# #(Hs & HΓ)"; iIntros (j K) "Hj /=".
-    smart_wp_bind (InjRCtx) v v' "[Hv #Hiv]"
-      (bin_log_related_alt _ _ j (InjRCtx :: K) with "IH"); cbn.
-    iApply wp_value. iExists (InjRV v'); iFrame "Hv".
-    iRight; iExists (_,_); eauto 10.
+    iIntros "#IH" (Δ vvs) "!# #(Hs & HΓ)".
+    iApply (bin_expr_rel_bind [InjRCtx] [InjRCtx]); first by iApply "IH"; iFrame "#".
+    iIntros (v v') "Hvv /=".
+    iApply (bin_val_rel_bin_expr_rel (InjRV _) (InjRV _)).
+    iRight; iExists (_, _); simpl; eauto.
   Qed.
 
   Lemma bin_log_related_case Γ e0 e1 e2 e0' e1' e2' τ1 τ2 τ3 :
@@ -138,25 +161,23 @@ Section fundamental.
     τ2 :: Γ ⊨ e2 ≤log≤ e2' : τ3 -∗
     Γ ⊨ Case e0 e1 e2 ≤log≤ Case e0' e1' e2' : τ3.
   Proof.
-    iIntros "#IH1 #IH2 #IH3" (Δ vvs) "!# #(Hs & HΓ)"; iIntros (j K) "Hj /=".
-    iDestruct (interp_env_length with "HΓ") as %?.
-    smart_wp_bind (CaseCtx _ _) v v' "[Hv #Hiv]"
-      (bin_log_related_alt _ _ j ((CaseCtx _ _) :: K) with "IH1"); cbn.
-    iDestruct "Hiv" as "[Hiv|Hiv]";
-    iDestruct "Hiv" as ([w w']) "[% Hw]"; simplify_eq.
-    - iApply fupd_wp.
-      iMod (step_case_inl with "[Hs Hv]") as "Hz"; eauto.
-      iApply wp_pure_step_later; auto. fold of_val. iModIntro. iNext.
-      asimpl.
-      iApply (bin_log_related_alt _ ((w,w') :: vvs) with "IH2").
-      repeat iSplit; eauto.
+    iIntros "#IH1 #IH2 #IH3" (Δ vvs) "!# #(Hs & HΓ)".
+    iApply (bin_expr_rel_bind [CaseCtx _ _] [CaseCtx _ _]); first by iApply "IH1"; iFrame "#".
+    iIntros (v v') "Hvv /=".
+    iDestruct "Hvv" as "[Hvv|Hvv]".
+    - iDestruct "Hvv" as ([w w']) "[% Hw]"; simplify_eq/=.
+      iIntros (M j K) "Hreg Hj /=".
+      iApply wp_pure_step_later; eauto. iNext.
+      iMod (step_case_inl with "[$]") as "Hj"; eauto.
+      iAsimpl.
+      iApply (bin_log_related_alt _ ((w,w') :: vvs) with "IH2"); iFrame; iFrame "#".
       iApply interp_env_cons; auto.
-    - iApply fupd_wp.
-      iMod (step_case_inr with "[Hs Hv]") as "Hz"; eauto.
-      iApply wp_pure_step_later; auto. fold of_val. iModIntro. iNext.
-      asimpl.
-      iApply (bin_log_related_alt _ ((w,w') :: vvs) with "IH3").
-      repeat iSplit; eauto.
+    - iDestruct "Hvv" as ([w w']) "[% Hw]"; simplify_eq/=.
+      iIntros (M j K) "Hreg Hj /=".
+      iApply wp_pure_step_later; eauto. iNext.
+      iMod (step_case_inr with "[$]") as "Hj"; eauto.
+      iAsimpl.
+      iApply (bin_log_related_alt _ ((w,w') :: vvs) with "IH3"); iFrame; iFrame "#".
       iApply interp_env_cons; auto.
   Qed.
 
@@ -166,17 +187,20 @@ Section fundamental.
     Γ ⊨ e2 ≤log≤ e2' : τ -∗
     Γ ⊨ If e0 e1 e2 ≤log≤ If e0' e1' e2' : τ.
   Proof.
-    iIntros "#IH1 #IH2 #IH3" (Δ vvs) "!# #(Hs & HΓ)"; iIntros (j K) "Hj /=".
-    smart_wp_bind (IfCtx _ _) v v' "[Hv #Hiv]"
-      (bin_log_related_alt _ _ j ((IfCtx _ _) :: K) with "IH1"); cbn.
-    iDestruct "Hiv" as ([]) "[% %]"; simplify_eq/=; iApply fupd_wp.
-    - iMod (step_if_true _ j K with "[-]") as "Hz"; eauto.
-      iApply wp_pure_step_later; auto. iModIntro. iNext.
-      iApply (bin_log_related_alt with "IH2"); eauto.
-    - iMod (step_if_false _ j K with "[-]") as "Hz"; eauto.
-      iApply wp_pure_step_later; auto.
-      iModIntro. iNext.
-      iApply (bin_log_related_alt with "IH3"); eauto.
+    iIntros "#IH1 #IH2 #IH3" (Δ vvs) "!# #(Hs & HΓ)".
+    iApply (bin_expr_rel_bind [IfCtx _ _] [IfCtx _ _]); first by iApply "IH1"; iFrame "#".
+    iIntros (v v') "Hvv /=".
+    iDestruct "Hvv" as ([]) "[-> ->]".
+    - iIntros (M j K) "Hreg Hj /=".
+      iApply wp_pure_step_later; eauto. iNext.
+      iMod (step_if_true with "[$]") as "Hj"; eauto.
+      iAsimpl.
+      iApply (bin_log_related_alt with "IH2"); iFrame; iFrame "#".
+    - iIntros (M j K) "Hreg Hj /=".
+      iApply wp_pure_step_later; eauto. iNext.
+      iMod (step_if_false with "[$]") as "Hj"; eauto.
+      iAsimpl.
+      iApply (bin_log_related_alt with "IH3"); iFrame; iFrame "#".
   Qed.
 
   Lemma bin_log_related_nat_binop Γ op e1 e2 e1' e2' :
@@ -184,17 +208,18 @@ Section fundamental.
     Γ ⊨ e2 ≤log≤ e2' : TNat -∗
     Γ ⊨ BinOp op e1 e2 ≤log≤ BinOp op e1' e2' : binop_res_type op.
   Proof.
-    iIntros "#IH1 #IH2" (Δ vvs) "!# #(Hs & HΓ)"; iIntros (j K) "Hj /=".
-    smart_wp_bind (BinOpLCtx _ _) v v' "[Hv #Hiv]"
-                  (bin_log_related_alt _ _ j ((BinOpLCtx _ _) :: K) with "IH1"); cbn.
-    smart_wp_bind (BinOpRCtx _ _) w w' "[Hw #Hiw]"
-                  (bin_log_related_alt _ _ j ((BinOpRCtx _ _) :: K) with "IH2"); cbn.
-    iDestruct "Hiv" as (n) "[% %]"; simplify_eq/=.
-    iDestruct "Hiw" as (n') "[% %]"; simplify_eq/=.
-    iApply fupd_wp.
-    iMod (step_nat_binop _ j K with "[-]") as "Hz"; eauto.
-    iApply wp_pure_step_later; auto. iModIntro. iNext.
-    iApply wp_value. iExists _; iSplitL; eauto.
+    iIntros "#IH1 #IH2" (Δ vvs) "!# #(Hs & HΓ)".
+    iApply (bin_expr_rel_bind [BinOpLCtx _ _] [BinOpLCtx _ _]); first by iApply "IH1"; iFrame "#".
+    iIntros (v v') "Hvv /=".
+    iDestruct "Hvv" as (n1) "[% %]"; simplify_eq/=.
+    iApply (bin_expr_rel_bind [BinOpRCtx _ (NatV _)] [BinOpRCtx _ (NatV _)]);
+        first by iApply "IH2"; iFrame "#".
+    iIntros (v v') "Hvv /=".
+    iDestruct "Hvv" as (n2) "[% %]"; simplify_eq/=.
+    iIntros (M j K) "Hreg Hj /=".
+    iApply wp_pure_step_later; eauto. iNext.
+    iMod (step_nat_binop _ j K with "[$]") as "Hj"; eauto.
+    iApply wp_value. iExists _, _; iFrame.
     destruct op; simpl; try destruct eq_nat_dec; try destruct le_dec;
       try destruct lt_dec; eauto.
   Qed.
@@ -203,36 +228,37 @@ Section fundamental.
     TArrow τ1 τ2 :: τ1 :: Γ ⊨ e ≤log≤ e' : τ2 -∗
     Γ ⊨ Rec e ≤log≤ Rec e' : TArrow τ1 τ2.
   Proof.
-    iIntros "#IH" (Δ vvs) "!# #(Hs & HΓ)"; iIntros (j K) "Hj /=".
-    iApply wp_value. iExists (RecV _). iIntros "{$Hj} !#".
-    iLöb as "IHL". iIntros ([v v']) "#Hiv". iIntros (j' K') "Hj".
+    iIntros "#IH" (Δ vvs) "!# #(Hs & HΓ)".
+    iApply (bin_val_rel_bin_expr_rel (RecV _) (RecV _)); simpl.
+    iIntros "!#".
+    iLöb as "IHL". iIntros ([v v']) "#Hiv /=".
     iDestruct (interp_env_length with "HΓ") as %?.
+    iIntros (M j K) "Hreg Hj /=".
     iApply wp_pure_step_later; auto 1 using to_of_val. iNext.
-    iApply fupd_wp.
-    iMod (step_rec _ j' K' _ (of_val v') v' with "[-]") as "Hz"; eauto.
-    asimpl. change (Rec ?e) with (of_val (RecV e)).
+    iMod (step_rec _ _ _ _ (of_val v') v' with "[$]") as "Hz"; eauto.
+    iAsimpl.
+    change (Rec ?e) with (of_val (RecV e)).
     iApply (bin_log_related_alt _ ((_,_) :: (v,v') :: vvs) with "IH").
-    repeat iSplit; eauto.
-    iModIntro.
-    rewrite !interp_env_cons; iSplit; try iApply interp_env_cons; auto.
+    iFrame; iFrame "#".
+    rewrite !interp_env_cons; eauto.
   Qed.
 
   Lemma bin_log_related_lam Γ e e' τ1 τ2 :
     τ1 :: Γ ⊨ e ≤log≤ e' : τ2 -∗
     Γ ⊨ Lam e ≤log≤ Lam e' : TArrow τ1 τ2.
   Proof.
-    iIntros "#IH" (Δ vvs) "!# #(Hs & HΓ)"; iIntros (j K) "Hj /=".
-    iApply wp_value. iExists (LamV _). iIntros "{$Hj} !#".
-    iIntros ([v v']) "#Hiv". iIntros (j' K') "Hj".
+    iIntros "#IH" (Δ vvs) "!# #(Hs & HΓ)".
+    iApply (bin_val_rel_bin_expr_rel (LamV _) (LamV _)); simpl.
+    iIntros "!#".
+    iIntros ([v v']) "#Hiv /=".
     iDestruct (interp_env_length with "HΓ") as %?.
+    iIntros (M j K) "Hreg Hj /=".
     iApply wp_pure_step_later; auto 1 using to_of_val. iNext.
-    iApply fupd_wp.
-    iMod (step_lam _ j' K' _ (of_val v') v' with "[-]") as "Hz"; eauto.
-    asimpl. iFrame "#". change (Lam ?e) with (of_val (LamV e)).
-    iApply (bin_log_related_alt _  ((v,v') :: vvs) with "IH").
-    repeat iSplit; eauto.
-    iModIntro.
-    rewrite !interp_env_cons; iSplit; try iApply interp_env_cons; auto.
+    iMod (step_lam _ _ _ _ (of_val v') v' with "[$]") as "Hz"; eauto.
+    iAsimpl.
+    iApply (bin_log_related_alt _ ((v,v') :: vvs) with "IH").
+    iFrame; iFrame "#".
+    rewrite !interp_env_cons; eauto.
   Qed.
 
   Lemma bin_log_related_letin Γ e1 e2 e1' e2' τ1 τ2 :
@@ -240,16 +266,17 @@ Section fundamental.
     τ1 :: Γ ⊨ e2 ≤log≤ e2' : τ2 -∗
     Γ ⊨ LetIn e1 e2 ≤log≤ LetIn e1' e2': τ2.
   Proof.
-    iIntros "#IH1 #IH2" (Δ vvs) "!# #(Hs & HΓ)"; iIntros (j K) "Hj /=".
+    iIntros "#IH1 #IH2" (Δ vvs) "!# #(Hs & HΓ)".
+    iApply (bin_expr_rel_bind [LetInCtx _] [LetInCtx _]); first by iApply "IH1"; iFrame "#".
+    iIntros (v v') "Hvv /=".
     iDestruct (interp_env_length with "HΓ") as %?.
-    smart_wp_bind (LetInCtx _) v v' "[Hv #Hiv]"
-      (bin_log_related_alt _ _ j ((LetInCtx _) :: K) with "IH1"); cbn.
-    iMod (step_letin _ j K with "[-]") as "Hz"; eauto.
+    iIntros (M j K) "Hreg Hj /=".
+    iMod (step_letin with "[$]") as "Hz"; eauto.
     iApply wp_pure_step_later; auto. iModIntro.
-    asimpl.
+    iAsimpl.
     iApply (bin_log_related_alt _ ((v, v') :: vvs) with "IH2").
-    repeat iSplit; eauto.
-    rewrite !interp_env_cons; iSplit; try iApply interp_env_cons; auto.
+    iFrame; iFrame "#".
+    rewrite !interp_env_cons; eauto.
   Qed.
 
   Lemma bin_log_related_seq Γ e1 e2 e1' e2' τ1 τ2 :
@@ -257,14 +284,14 @@ Section fundamental.
     Γ ⊨ e2 ≤log≤ e2' : τ2 -∗
     Γ ⊨ Seq e1 e2 ≤log≤ Seq e1' e2': τ2.
   Proof.
-    iIntros "#IH1 #IH2" (Δ vvs) "!# #(Hs & HΓ)"; iIntros (j K) "Hj /=".
-    iDestruct (interp_env_length with "HΓ") as %?.
-    smart_wp_bind (SeqCtx _) v v' "[Hv #Hiv]"
-      (bin_log_related_alt _ _ j ((SeqCtx _) :: K) with "IH1"); cbn.
-    iMod (step_seq _ j K with "[-]") as "Hz"; eauto.
+    iIntros "#IH1 #IH2" (Δ vvs) "!# #(Hs & HΓ)".
+    iApply (bin_expr_rel_bind [SeqCtx _] [SeqCtx _]); first by iApply "IH1"; iFrame "#".
+    iIntros (v v') "Hvv /=".
+    iIntros (M j K) "Hreg Hj /=".
+    iMod (step_seq with "[$]") as "Hz"; eauto.
     iApply wp_pure_step_later; auto. iModIntro.
-    asimpl.
-    iApply (bin_log_related_alt with "IH2"); repeat iSplit; eauto.
+    iApply (bin_log_related_alt with "IH2").
+    iFrame; iFrame "#".
   Qed.
 
   Lemma bin_log_related_app Γ e1 e2 e1' e2' τ1 τ2 :
@@ -272,54 +299,48 @@ Section fundamental.
     Γ ⊨ e2 ≤log≤ e2' : τ1 -∗
     Γ ⊨ App e1 e2 ≤log≤ App e1' e2' :  τ2.
   Proof.
-    iIntros "#IH1 #IH2" (Δ vvs) "!# #(Hs & HΓ)"; iIntros (j K) "Hj /=".
-    smart_wp_bind (AppLCtx (e2.[env_subst (vvs.*1)])) v v' "[Hv #Hiv]"
-      (bin_log_related_alt
-        _ _ j (((AppLCtx (e2'.[env_subst (vvs.*2)]))) :: K) with "IH1"); cbn.
-    smart_wp_bind (AppRCtx v) w w' "[Hw #Hiw]"
-      (bin_log_related_alt _ _ j ((AppRCtx v') :: K) with "IH2"); cbn.
-    iApply ("Hiv" $! (w, w') with "Hiw"); simpl; eauto.
+    iIntros "#IH1 #IH2" (Δ vvs) "!# #(Hs & HΓ)".
+    iApply (bin_expr_rel_bind [AppLCtx _] [AppLCtx _]); first by iApply "IH1"; iFrame "#".
+    iIntros (v v') "Hvv /=".
+    iApply (bin_expr_rel_bind [AppRCtx _] [AppRCtx _]); first by iApply "IH2"; iFrame "#".
+    iIntros (w w') "Hww /=".
+    iIntros (M j K) "Hreg Hj /=".
+    iApply ("Hvv" $! (w, w') with "[$] Hreg"); iFrame.
   Qed.
 
   Lemma bin_log_related_tlam Γ e e' τ :
     (subst (ren (+1)) <$> Γ) ⊨ e ≤log≤ e' : τ -∗
     Γ ⊨ TLam e ≤log≤ TLam e' : TForall τ.
   Proof.
-    iIntros "#IH" (Δ vvs) "!# #(Hs & HΓ)"; iIntros (j K) "Hj /=".
-    iApply wp_value. iExists (TLamV _).
-    iIntros "{$Hj} /= !#"; iIntros (τi j' K') "Hv /=".
+    iIntros "#IH" (Δ vvs) "!# #(Hs & HΓ)".
+    iApply (bin_val_rel_bin_expr_rel (TLamV _) (TLamV _)); simpl.
+    iIntros "!#"; iIntros (τi M j K) "Hreg Hj /=".
     iApply wp_pure_step_later; auto. iNext.
-    iApply fupd_wp.
-    iMod (step_tlam _ j' K' (e'.[env_subst (vvs.*2)]) with "[-]") as "Hz"; eauto.
-    iApply (bin_log_related_alt with "IH"); repeat iSplit; eauto.
-    iModIntro.
+    iMod (step_tlam with "[$]") as "Hj"; eauto.
+    iApply (bin_log_related_alt with "IH [$Hj $Hreg]"); iFrame "#"; [].
     rewrite interp_env_ren; auto.
   Qed.
 
   Lemma bin_log_related_tapp Γ e e' τ τ' :
     Γ ⊨ e ≤log≤ e' : TForall τ -∗ Γ ⊨ TApp e ≤log≤ TApp e' : τ.[τ'/].
   Proof.
-    iIntros "#IH" (Δ vvs) "!# #(Hs & HΓ)"; iIntros (j K) "Hj /=".
-    smart_wp_bind (TAppCtx) v v' "[Hj #Hv]"
-      (bin_log_related_alt _ _ j (TAppCtx :: K) with "IH"); cbn.
-    rewrite -/interp.
-    iApply wp_wand_r; iSplitL.
-    { iSpecialize ("Hv" $! (interp τ' Δ)). iApply "Hv"; eauto. }
-    iIntros (w). iDestruct 1 as (w') "[Hw Hiw]".
-    iExists _; rewrite -interp_subst; eauto.
+    iIntros "#IH" (Δ vvs) "!# #(Hs & HΓ)"; simpl.
+    iApply (bin_expr_rel_bind [TAppCtx] [TAppCtx]); first by iApply "IH"; iFrame "#".
+    iIntros (v v') "Hvv /=".
+    iApply interp_expr_change_type; first by intros; rewrite -interp_subst.
+    iApply "Hvv".
   Qed.
 
   Lemma bin_log_related_pack Γ e e' τ τ' :
     Γ ⊨ e ≤log≤ e' : τ.[τ'/] -∗ Γ ⊨ Pack e ≤log≤ Pack e' : TExist τ.
   Proof.
-    iIntros "#IH" (Δ vvs) "!# #(Hs & HΓ)"; iIntros (j K) "Hj /=".
-    smart_wp_bind (PackCtx) v v' "[Hj #Hv]"
-      (bin_log_related_alt _ _ j (PackCtx :: K) with "IH"); cbn.
-    iApply wp_value.
-    iExists (PackV _); iFrame.
-    iModIntro.
+    iIntros "#IH" (Δ vvs) "!# #(Hs & HΓ)".
+    iApply (bin_expr_rel_bind [PackCtx] [PackCtx]); first by iApply "IH"; iFrame "#".
+    iIntros (v v') "#Hvv /=".
+    iApply (bin_val_rel_bin_expr_rel (PackV _) (PackV _)).
     rewrite -interp_subst.
-    iExists (interp _ Δ), (_, _); iSplit; done.
+    iIntros "!#".
+    iExists _, (_, _); iSplit; done.
   Qed.
 
   Lemma bin_log_related_unpack Γ e1 e1' e2 e2' τ τ' :
@@ -327,35 +348,32 @@ Section fundamental.
     τ :: (subst (ren (+1)) <$> Γ) ⊨ e2 ≤log≤ e2' : τ'.[ren (+1)] -∗
     Γ ⊨ UnpackIn e1 e2 ≤log≤ UnpackIn e1' e2' : τ'.
   Proof.
-    iIntros "#IH1 #IH2" (Δ vvs) "!# #(Hs & HΓ)"; iIntros (j K) "Hj /=".
-    smart_wp_bind (UnpackInCtx _) v v' "[Hj #Hv]"
-      (bin_log_related_alt _ _ j (UnpackInCtx _ :: K) with "IH1"); cbn.
-    rewrite -/interp.
-    iDestruct "Hv" as (τi (v1, v2) Hvv) "#Hvv"; simplify_eq /=.
+    iIntros "#IH1 #IH2" (Δ vvs) "!# #(Hs & HΓ)".
+    iApply (bin_expr_rel_bind [UnpackInCtx _] [UnpackInCtx _]); first by iApply "IH1"; iFrame "#".
+    simpl.
+    iIntros (v v') "#Hvv /=".
+    iDestruct "Hvv" as (τi (v1, v2) ?) "Hvv"; simplify_eq/=.
+    iIntros (M j K) "Hreg Hj /=".
     iApply wp_pure_step_later; auto. iNext.
-    iApply fupd_wp.
-    iMod (step_pack with "[Hj]") as "Hj"; eauto.
-    asimpl.
-    iModIntro.
+    iMod (step_pack with "[$]") as "Hj"; eauto.
+    iAsimpl.
     iApply wp_wand_r; iSplitL.
-    { iApply (bin_log_related_alt (τi :: Δ) ((v1, v2) :: vvs) with "IH2 [$Hj]").
-      iFrame; iFrame "#".
+    { iApply (bin_log_related_alt (τi :: Δ) ((v1, v2) :: vvs) with "IH2 [$Hj $Hreg]").
+      iFrame "#".
       iApply interp_env_cons; iSplit; first done.
       by iApply interp_env_ren. }
-    iIntros (w). iDestruct 1 as (v) "[Hj #Hv]".
-    iExists _; iFrame.
+    iIntros (w). iDestruct 1 as (v M') "[Hreg [Hj #Hv]]".
+    iExists _, _; iFrame.
     by iApply (interp_weaken [] [_]); simpl.
   Qed.
 
   Lemma bin_log_related_fold Γ e e' τ :
     Γ ⊨ e ≤log≤ e' : τ.[(TRec τ)/] -∗ Γ ⊨ Fold e ≤log≤ Fold e' : TRec τ.
   Proof.
-    iIntros "#IH" (Δ vvs) "!# #(Hs & HΓ)"; iIntros (j K) "Hj /=".
-    iApply (wp_bind (fill [FoldCtx])); iApply wp_wand_l; iSplitR;
-        [|iApply (bin_log_related_alt _ _ j (FoldCtx :: K) with "IH");
-          simpl; repeat iSplitR; trivial].
-    iIntros (v); iDestruct 1 as (w) "[Hv #Hiv]".
-    iApply wp_value. iExists (FoldV w); iFrame "Hv".
+    iIntros "#IH" (Δ vvs) "!# #(Hs & HΓ)".
+    iApply (bin_expr_rel_bind [FoldCtx] [FoldCtx]); first by iApply "IH"; iFrame "#".
+    iIntros (v v') "#Hvv /=".
+    iApply (bin_val_rel_bin_expr_rel (FoldV _) (FoldV _)).
     rewrite fixpoint_interp_rec1_eq /= -interp_subst.
     iModIntro; iExists (_, _); eauto.
   Qed.
@@ -363,56 +381,50 @@ Section fundamental.
   Lemma bin_log_related_unfold Γ e e' τ :
     Γ ⊨ e ≤log≤ e' : TRec τ -∗ Γ ⊨ Unfold e ≤log≤ Unfold e' : τ.[(TRec τ)/].
   Proof.
-    iIntros "#IH" (Δ vvs) "!# #(Hs & HΓ)"; iIntros (j K) "Hj /=".
-    iApply (wp_bind (fill [UnfoldCtx])); iApply wp_wand_l; iSplitR;
-        [|iApply (bin_log_related_alt _ _ j (UnfoldCtx :: K) with "IH");
-          simpl; repeat iSplitR; trivial].
-    iIntros (v). iDestruct 1 as (v') "[Hw #Hiw]".
-    rewrite /= fixpoint_interp_rec1_eq /=.
-    change (fixpoint _) with (interp (TRec τ) Δ).
-    iDestruct "Hiw" as ([w w']) "#[% Hiz]"; simplify_eq/=.
-    iApply fupd_wp.
-    iMod (step_fold _ j K (of_val w') w' with "[-]") as "Hz"; eauto.
+    iIntros "#IH" (Δ vvs) "!# #(Hs & HΓ)".
+    iApply (bin_expr_rel_bind [UnfoldCtx] [UnfoldCtx]); first by iApply "IH"; iFrame "#".
+    iIntros (v v') "#Hvv /=".
+    rewrite fixpoint_interp_rec1_eq /=.
+    iDestruct "Hvv" as ([]) "[% #Hvv]"; simplify_eq/=.
+    iIntros (M j K) "Hreg Hj /=".
+    iMod (step_fold with "[$]") as "Hj"; eauto.
     iApply wp_pure_step_later; auto.
-    iModIntro. iApply wp_value. iNext; iExists _; iFrame "Hz".
-      by rewrite -interp_subst.
+    iApply wp_value; iNext. iExists _, _; iFrame.
+    by rewrite -interp_subst.
   Qed.
 
   Lemma bin_log_related_alloc Γ e e' τ :
       Γ ⊨ e ≤log≤ e' : τ -∗ Γ ⊨ Alloc e ≤log≤ Alloc e' : Tref τ.
   Proof.
-    iIntros "#IH" (Δ vvs) "!# #(Hs & HΓ)"; iIntros (j K) "Hj /=".
-    smart_wp_bind (AllocCtx) v v' "[Hv #Hiv]"
-      (bin_log_related_alt _ _ j (AllocCtx :: K) with "IH").
-    iApply fupd_wp.
-    iMod (step_alloc _ j K (of_val v') v' with "[-]") as (l') "[Hj Hl]"; eauto.
-    iApply wp_atomic; eauto.
-    iApply wp_alloc; eauto. do 2 iModIntro. iNext.
+    iIntros "#IH" (Δ vvs) "!# #(Hs & HΓ)".
+    iApply (bin_expr_rel_bind [AllocCtx] [AllocCtx]); first by iApply "IH"; iFrame "#".
+    iIntros (v v') "#Hvv /=".
+    iIntros (M j K) "Hreg Hj /=".
+    iMod (step_alloc with "[$]") as (l') "[Hj Hl]"; eauto.
+    iApply wp_fupd.
+    iApply wp_alloc; eauto. iNext.
     iIntros (l) "Hl'".
     iMod (inv_alloc (logN .@ (l,l')) _ (∃ w : val * val,
       l ↦ᵢ w.1 ∗ l' ↦ₛ w.2 ∗ interp τ Δ w)%I with "[Hl Hl']") as "HN"; eauto.
-    { iNext. iExists (v, v'); iFrame. iFrame "Hiv". }
-    iModIntro; iExists (LocV l'). iFrame "Hj". iExists (l, l'); eauto.
+    { by iNext; iExists (v, v'); iFrame. }
+    iModIntro; iExists (LocV l'), _. iFrame. iExists (l, l'); eauto.
   Qed.
 
   Lemma bin_log_related_load Γ e e' τ :
     Γ ⊨ e ≤log≤ e' : (Tref τ) -∗ Γ ⊨ Load e ≤log≤ Load e' : τ.
   Proof.
-    iIntros "#IH" (Δ vvs) "!# #(Hs & HΓ)"; iIntros (j K) "Hj /=".
-    smart_wp_bind (LoadCtx) v v' "[Hv #Hiv]"
-      (bin_log_related_alt _ _ j (LoadCtx :: K) with "IH").
-    iDestruct "Hiv" as ([l l']) "[% Hinv]"; simplify_eq/=.
-    iApply wp_atomic; eauto.
+    iIntros "#IH" (Δ vvs) "!# #(Hs & HΓ)".
+    iApply (bin_expr_rel_bind [LoadCtx] [LoadCtx]); first by iApply "IH"; iFrame "#".
+    iIntros (v v') "#Hvv /=".
+    iDestruct "Hvv" as ([l l']) "[% Hinv]"; simplify_eq/=.
+    iIntros (M j K) "Hreg Hj /=".
     iInv (logN .@ (l,l')) as ([w w']) "[Hw1 [>Hw2 #Hw]]" "Hclose"; simpl.
-    (* TODO: why can we eliminate the next modality here? ↑ *)
-    iModIntro.
     iApply (wp_load with "Hw1").
     iNext. iIntros "Hw1".
-    iMod (step_load  with "[Hv Hw2]") as "[Hv Hw2]";
-      [solve_ndisj|by iFrame|].
-    iMod ("Hclose" with "[Hw1 Hw2]").
+    iMod (step_load  with "[$]") as "[Hv Hw2]"; first by solve_ndisj.
+    iMod ("Hclose" with "[Hw1 Hw2]") as "_".
     { iNext. iExists (w,w'); by iFrame. }
-    iModIntro. iExists w'; by iFrame.
+    iModIntro. iExists w', _; by iFrame.
   Qed.
 
   Lemma bin_log_related_store Γ e1 e2 e1' e2' τ :
@@ -420,53 +432,52 @@ Section fundamental.
     Γ ⊨ e2 ≤log≤ e2' : τ -∗
     Γ ⊨ Store e1 e2 ≤log≤ Store e1' e2' : TUnit.
   Proof.
-    iIntros "#IH1 #IH2" (Δ vvs) "!# #(Hs & HΓ)"; iIntros (j K) "Hj /=".
-    smart_wp_bind (StoreLCtx _) v v' "[Hv #Hiv]"
-      (bin_log_related_alt _ _ j ((StoreLCtx _) :: K) with "IH1").
-    smart_wp_bind (StoreRCtx _) w w' "[Hw #Hiw]"
-      (bin_log_related_alt _ _ j ((StoreRCtx _) :: K) with "IH2").
-    iDestruct "Hiv" as ([l l']) "[% Hinv]"; simplify_eq/=.
-    iApply wp_atomic; eauto.
+    iIntros "#IH1 #IH2" (Δ vvs) "!# #(Hs & HΓ)".
+    iApply (bin_expr_rel_bind [StoreLCtx _] [StoreLCtx _]); first by iApply "IH1"; iFrame "#".
+    iIntros (v v') "#Hvv /=".
+    iDestruct "Hvv" as ([l l']) "[% Hinv]"; simplify_eq/=.
+    iApply (bin_expr_rel_bind [StoreRCtx (LocV _)] [StoreRCtx (LocV _)]);
+        first by iApply "IH2"; iFrame "#".
+    iIntros (w w') "#Hww/=".
+    iIntros (M j K) "Hreg Hj /=".
     iInv (logN .@ (l,l')) as ([v v']) "[Hv1 [>Hv2 #Hv]]" "Hclose".
-    iModIntro.
     iApply (wp_store with "Hv1"); auto using to_of_val.
     iNext. iIntros "Hw2".
-    iMod (step_store with "[$Hs Hw Hv2]") as "[Hw Hv2]"; eauto;
-    [solve_ndisj | by iFrame|].
-    iMod ("Hclose" with "[Hw2 Hv2]").
-    { iNext; iExists (w, w'); simpl; iFrame. iFrame "Hiw". }
+    iMod (step_store with "[$]") as "[Hw Hv2]"; eauto; first by solve_ndisj.
+    iMod ("Hclose" with "[Hw2 Hv2]") as "_".
+    { by iNext; iExists (w, w'); simpl; iFrame. }
     iExists UnitV; iFrame; auto.
   Qed.
 
   Theorem binary_fundamental Γ e τ :
     Γ ⊢ₜ e : τ → ⊢ Γ ⊨ e ≤log≤ e : τ.
   Proof.
-    induction 1.
+    revert Γ e τ; fix IH 4; destruct 1.
     - iApply bin_log_related_var; done.
     - iApply bin_log_related_unit.
     - iApply bin_log_related_nat.
     - iApply bin_log_related_bool.
-    - iApply bin_log_related_nat_binop; done.
-    - iApply bin_log_related_pair; done.
-    - iApply bin_log_related_fst; done.
-    - iApply bin_log_related_snd; done.
-    - iApply bin_log_related_injl; done.
-    - iApply bin_log_related_injr; done.
-    - iApply bin_log_related_case; done.
-    - iApply bin_log_related_if; done.
-    - iApply bin_log_related_rec; done.
-    - iApply bin_log_related_lam; done.
-    - iApply bin_log_related_letin; done.
-    - iApply bin_log_related_seq; done.
-    - iApply bin_log_related_app; done.
-    - iApply bin_log_related_tlam; done.
-    - iApply bin_log_related_tapp; done.
-    - iApply bin_log_related_pack; done.
-    - iApply bin_log_related_unpack; done.
-    - iApply bin_log_related_fold; done.
-    - iApply bin_log_related_unfold; done.
-    - iApply bin_log_related_alloc; done.
-    - iApply bin_log_related_load; done.
-    - iApply bin_log_related_store; done.
+    - iApply bin_log_related_nat_binop; iApply IH; done.
+    - iApply bin_log_related_pair; iApply IH; done.
+    - iApply bin_log_related_fst; iApply IH; done.
+    - iApply bin_log_related_snd; iApply IH; done.
+    - iApply bin_log_related_injl; iApply IH; done.
+    - iApply bin_log_related_injr; iApply IH; done.
+    - iApply bin_log_related_case; iApply IH; done.
+    - iApply bin_log_related_if; iApply IH; done.
+    - iApply bin_log_related_rec; iApply IH; done.
+    - iApply bin_log_related_lam; iApply IH; done.
+    - iApply bin_log_related_letin; iApply IH; done.
+    - iApply bin_log_related_seq; iApply IH; done.
+    - iApply bin_log_related_app; iApply IH; done.
+    - iApply bin_log_related_tlam; iApply IH; done.
+    - iApply bin_log_related_tapp; iApply IH; done.
+    - iApply bin_log_related_pack; iApply IH; done.
+    - iApply bin_log_related_unpack; iApply IH; done.
+    - iApply bin_log_related_fold; iApply IH; done.
+    - iApply bin_log_related_unfold; iApply IH; done.
+    - iApply bin_log_related_alloc; iApply IH; done.
+    - iApply bin_log_related_load; iApply IH; done.
+    - iApply bin_log_related_store; iApply IH; done.
   Qed.
 End fundamental.
