theories/F_mu_ref/unary/fundamental.v
@@ -5,12 +5,12 @@ From WBLogrel.F_mu_ref.unary Require Export logrel.
 From WBLogrel.F_mu_ref Require Export rules.
 From iris.prelude Require Import options.
 
-Definition log_typed `{heapIG Σ} (Γ : list type) (e : expr) (τ : type) : iProp Σ :=
+Definition log_typed `{heapIG Σ, ghost_regG Σ} (Γ : list type) (e : expr) (τ : type) : iProp Σ :=
   □ ∀ Δ vs, ⟦ Γ ⟧* Δ vs -∗ ⟦ τ ⟧ₑ Δ e.[env_subst vs].
 Notation "Γ ⊨ e : τ" := (log_typed Γ e τ) (at level 74, e, τ at next level).
 
 Section typed_interp.
-  Context `{heapIG Σ}.
+  Context `{heapIG Σ, ghost_regG Σ}.
   Notation D := (persistent_predO val (iPropI Σ)).
 
   Local Tactic Notation "smart_wp_bind"
@@ -25,26 +25,39 @@ Section typed_interp.
     iIntros (? Δ vs) "!# #HΓ"; simpl.
     iDestruct (interp_env_Some_l with "HΓ") as (v) "[% ?]"; first done.
     erewrite env_subst_lookup; eauto.
-    iApply wp_value; done.
+    iIntros (?) "?"; iApply wp_value; iExists _; iFrame; iSplit; done.
   Qed.
 
   Lemma sem_typed_unit Γ : ⊢ Γ ⊨ Unit : TUnit.
-  Proof. iIntros (Δ vs) "!# #HΓ". iApply wp_value; done. Qed.
+  Proof.
+    iIntros (Δ vs) "!# #HΓ".
+    iIntros (?) "?"; iApply wp_value; iExists _; iFrame; iSplit; done.
+  Qed.
 
   Lemma sem_typed_nat Γ n : ⊢ Γ ⊨ #n n : TNat.
-  Proof. iIntros (Δ vs) "!# #HΓ /=". iApply wp_value; eauto. Qed.
+  Proof.
+    iIntros (Δ vs) "!# #HΓ /=".
+    iIntros (?) "?"; iApply wp_value; iExists _; iFrame; iSplit; eauto.
+  Qed.
 
   Lemma sem_typed_bool Γ b : ⊢ Γ ⊨ #♭ b : TBool.
-  Proof. iIntros (Δ vs) "!# #HΓ /=". iApply wp_value; eauto. Qed.
+  Proof.
+    iIntros (Δ vs) "!# #HΓ /=".
+    iIntros (?) "?"; iApply wp_value; iExists _; iFrame; iSplit; eauto.
+  Qed.
 
   Lemma sem_typed_nat_binop Γ op e1 e2 :
     Γ ⊨ e1 : TNat -∗ Γ ⊨ e2 : TNat -∗ Γ ⊨ BinOp op e1 e2 : binop_res_type op.
   Proof.
     iIntros "#IH1 #IH2" (Δ vs) "!# #HΓ /=".
-    smart_wp_bind (BinOpLCtx _ e2.[env_subst vs]) v "#Hv" "IH1".
-    smart_wp_bind (BinOpRCtx _ v) v' "# Hv'" "IH2".
-    iDestruct "Hv" as (n) "%"; iDestruct "Hv'" as (n') "%"; simplify_eq/=.
+    iIntros (?) "?".
+    smart_wp_bind (BinOpLCtx _ e2.[env_subst vs]) v "Hv" "IH1".
+    iDestruct "Hv" as (N1 [] ?) "?".
+    smart_wp_bind (BinOpRCtx _ v) v' "Hv'" "IH2".
+    iDestruct "Hv'" as (N2 [] ?) "?".
+    simplify_eq/=.
     iApply wp_pure_step_later; auto. iNext. iApply wp_value.
+    iExists _; iSplit; last (iSplit; last (by iFrame); iPureIntro; etrans; done).
     destruct op; simpl; try destruct eq_nat_dec;
       try destruct le_dec; try destruct lt_dec; eauto 10.
   Qed.
@@ -53,41 +66,66 @@ Section typed_interp.
     Γ ⊨ e1 : τ1 -∗ Γ ⊨ e2 : τ2 -∗ Γ ⊨ Pair e1 e2 : TProd τ1 τ2.
   Proof.
     iIntros "#IH1 #IH2" (Δ vs) "!# #HΓ"; simpl.
-    smart_wp_bind (PairLCtx e2.[env_subst vs]) v "#Hv" "IH1".
-    smart_wp_bind (PairRCtx v) v' "# Hv'" "IH2".
-    iApply wp_value; eauto.
+    iIntros (?) "?".
+    smart_wp_bind (PairLCtx e2.[env_subst vs]) v "Hv" "IH1".
+    iDestruct "Hv" as (N1) "(#?&%&?)".
+    smart_wp_bind (PairRCtx v) v' "Hv'" "IH2".
+    iDestruct "Hv'" as (N2) "(#?&%&?)".
+    iApply wp_value.
+    iExists _; iSplit; last (iSplit; last (by iFrame); iPureIntro; etrans; done).
+    eauto.
   Qed.
 
   Lemma sem_typed_fst Γ e τ1 τ2 :
         Γ ⊨ e : TProd τ1 τ2 -∗ Γ ⊨ Fst e : τ1.
   Proof.
     iIntros "#IH" (Δ vs) "!# #HΓ"; simpl.
-    smart_wp_bind (FstCtx) v "# Hv" "IH"; cbn.
+    iIntros (?) "?".
+    smart_wp_bind (FstCtx) v "Hv" "IH"; cbn.
+    iDestruct "Hv" as (N1) "(#Hv&%&?)".
     iDestruct "Hv" as (w1 w2) "#[% [H2 H3]]"; subst.
-    iApply wp_pure_step_later; auto. by iApply wp_value.
+    simpl.
+    iApply wp_pure_step_later; auto.
+    iApply wp_value.
+    iExists _; iSplit; last (iSplit; last (by iFrame); iPureIntro; etrans; done).
+    done.
   Qed.
 
   Lemma sem_typed_snd Γ e τ1 τ2 :
     Γ ⊨ e : TProd τ1 τ2 -∗ Γ ⊨ Snd e : τ2.
   Proof.
     iIntros "#IH" (Δ vs) "!# #HΓ"; simpl.
-    smart_wp_bind (SndCtx) v "# Hv" "IH"; cbn.
+    iIntros (?) "?".
+    smart_wp_bind (SndCtx) v "Hv" "IH"; cbn.
+    iDestruct "Hv" as (N1) "(#Hv&%&?)".
     iDestruct "Hv" as (w1 w2) "#[% [H2 H3]]"; subst.
-    iApply wp_pure_step_later; auto. by iApply wp_value.
+    simpl.
+    iApply wp_pure_step_later; auto.
+    iApply wp_value.
+    iExists _; iSplit; last (iSplit; last (by iFrame); iPureIntro; etrans; done).
+    done.
   Qed.
 
   Lemma sem_typed_injl Γ e τ1 τ2 : Γ ⊨ e : τ1 -∗ Γ ⊨ InjL e : (TSum τ1 τ2).
   Proof.
     iIntros "#IH" (Δ vs) "!# #HΓ"; simpl.
-    smart_wp_bind (InjLCtx) v "# Hv" "IH"; cbn.
-    iApply wp_value; eauto.
+    iIntros (?) "?".
+    smart_wp_bind (InjLCtx) v "Hv" "IH"; cbn.
+    iDestruct "Hv" as (N1) "(#Hv&%&?)".
+    iApply wp_value.
+    iExists _; iSplit; last (iSplit; last (by iFrame); iPureIntro; etrans; done).
+    eauto.
   Qed.
 
   Lemma sem_typed_injr Γ e τ1 τ2 : Γ ⊨ e : τ2 -∗ Γ ⊨ InjR e : TSum τ1 τ2.
   Proof.
     iIntros "#IH" (Δ vs) "!# #HΓ"; simpl.
-    smart_wp_bind (InjRCtx) v "# Hv" "IH"; cbn.
-    iApply wp_value; eauto.
+    iIntros (?) "?".
+    smart_wp_bind (InjRCtx) v "Hv" "IH"; cbn.
+    iDestruct "Hv" as (N1) "(#Hv&%&?)".
+    iApply wp_value.
+    iExists _; iSplit; last (iSplit; last (by iFrame); iPureIntro; etrans; done).
+    eauto.
   Qed.
 
   Lemma sem_typed_case Γ e0 e1 e2 τ1 τ2 τ3 :
@@ -97,41 +135,68 @@ Section typed_interp.
     Γ ⊨ Case e0 e1 e2 : τ3.
   Proof.
     iIntros "#IH1 #IH2 #IH3" (Δ vs) "!# #HΓ"; simpl.
-    smart_wp_bind (CaseCtx _ _) v "#Hv" "IH1"; cbn.
+    iIntros (?) "?".
+    smart_wp_bind (CaseCtx _ _) v "Hv" "IH1"; cbn.
+    iDestruct "Hv" as (N1) "(#Hv&%&Hreg)".
     iDestruct (interp_env_length with "HΓ") as %?.
     iDestruct "Hv" as "[Hv|Hv]"; iDestruct "Hv" as (w) "[% Hw]"; simplify_eq/=.
-    + iApply wp_pure_step_later; auto 1 using to_of_val; asimpl. iNext.
-      iApply ("IH2" $! Δ (w :: vs)). iApply interp_env_cons; auto.
-    + iApply wp_pure_step_later; auto 1 using to_of_val; asimpl. iNext.
-      iApply ("IH3" $! Δ (w :: vs)). iApply interp_env_cons; auto.
+    + iApply wp_pure_step_later; first done. asimpl. iNext.
+      iApply (wp_wand with "[Hreg]"); first
+        iApply ("IH2" $! Δ (w :: vs) with "[] Hreg"); first by iApply interp_env_cons; auto.
+      iIntros (v). iDestruct 1 as (N) "(?&%&?)".
+      iExists _; iFrame; iPureIntro.
+      etrans; done.
+    + iApply wp_pure_step_later; first done. asimpl. iNext.
+      iApply (wp_wand with "[Hreg]"); first
+        iApply ("IH3" $! Δ (w :: vs) with "[] Hreg"); first by iApply interp_env_cons; auto.
+      iIntros (v). iDestruct 1 as (N) "(?&%&?)".
+      iExists _; iFrame; iPureIntro.
+      etrans; done.
   Qed.
 
   Lemma sem_typed_if Γ e0 e1 e2 τ :
     Γ ⊨ e0 : TBool -∗ Γ ⊨ e1 : τ -∗ Γ ⊨ e2 : τ -∗ Γ ⊨ If e0 e1 e2 : τ.
   Proof.
     iIntros "#IH1 #IH2 #IH3" (Δ vs) "!# #HΓ"; simpl.
-    smart_wp_bind (IfCtx _ _) v "#Hv" "IH1"; cbn.
+    iIntros (?) "?".
+    smart_wp_bind (IfCtx _ _) v "Hv" "IH1"; cbn.
+    iDestruct "Hv" as (N1) "(#Hv&%&Hreg)".
     iDestruct "Hv" as ([]) "%"; subst; simpl;
-      [iApply wp_pure_step_later .. ]; auto; iNext;
-        [iApply "IH2"| iApply "IH3"]; auto.
+      [iApply wp_pure_step_later .. ]; auto; iNext.
+    - iApply (wp_wand with "[Hreg]"); first
+        iApply ("IH2" with "[] Hreg"); first done.
+      iIntros (v). iDestruct 1 as (N) "(?&%&?)".
+      iExists _; iFrame; iPureIntro.
+      etrans; done.
+    - iApply (wp_wand with "[Hreg]"); first
+        iApply ("IH3" with "[] Hreg"); first done.
+      iIntros (v). iDestruct 1 as (N) "(?&%&?)".
+      iExists _; iFrame; iPureIntro.
+      etrans; done.
   Qed.
 
   Lemma sem_typed_rec Γ e τ1 τ2 :
     TArrow τ1 τ2 :: τ1 :: Γ ⊨ e : τ2 -∗ Γ ⊨ Rec e : TArrow τ1 τ2.
   Proof.
     iIntros "#IH" (Δ vs) "!# #HΓ"; simpl.
-    iApply wp_value. simpl. iModIntro. iLöb as "IHL". iIntros (w) "#Hw".
+    iIntros (?) "?".
+    iApply wp_value. simpl.
+    iExists _; iFrame; iSplit; last done.
+    iModIntro. iLöb as "IHL". iIntros (M' w) "Hreg #Hw".
     iDestruct (interp_env_length with "HΓ") as %?.
     iApply wp_pure_step_later; auto 1 using to_of_val. iNext.
     asimpl. change (Rec _) with (of_val (RecV e.[upn 2 (env_subst vs)])) at 2.
-    iApply ("IH" $! Δ (_ :: w :: vs)).
+    iApply ("IH" $! Δ (_ :: w :: vs)); last done.
     iApply interp_env_cons; iSplit; [|iApply interp_env_cons]; auto.
   Qed.
 
   Lemma sem_typed_lam Γ e τ1 τ2 : τ1 :: Γ ⊨ e : τ2 -∗ Γ ⊨ Lam e : TArrow τ1 τ2.
   Proof.
     iIntros "#IH" (Δ vs) "!# #HΓ"; simpl.
-    iApply wp_value. simpl. iModIntro. iIntros (w) "#Hw".
+    iIntros (?) "?".
+    iApply wp_value. simpl.
+    iExists _; iFrame; iSplit; last done.
+    iModIntro. iIntros (M' w) "Hreg #Hw".
     iDestruct (interp_env_length with "HΓ") as %?.
     iApply wp_pure_step_later; auto 1 using to_of_val. iNext.
     asimpl.
@@ -143,55 +208,86 @@ Section typed_interp.
     Γ ⊨ e1 : τ1 -∗ τ1 :: Γ ⊨ e2 : τ2 -∗ Γ ⊨ LetIn e1 e2: τ2.
   Proof.
     iIntros "#IH1 #IH2" (Δ vs) "!# #HΓ"; simpl.
-    smart_wp_bind (LetInCtx _) v "#Hv" "IH1"; cbn.
+    iIntros (?) "?".
+    smart_wp_bind (LetInCtx _) v "Hv" "IH1"; cbn.
+    iDestruct "Hv" as (N1) "(#Hv&%&Hreg)".
     iDestruct (interp_env_length with "HΓ") as %?.
     iApply wp_pure_step_later; auto 1 using to_of_val. iNext.
-    asimpl. iApply ("IH2" $! Δ (v :: vs)).
-    iApply interp_env_cons; iSplit; eauto.
+    asimpl.
+    iApply (wp_wand with "[Hreg]");
+      first iApply ("IH2" $! Δ (v :: vs) with "[] Hreg");
+      first by iApply interp_env_cons; iSplit; eauto.
+    iIntros (w). iDestruct 1 as (N2) "(?&%&?)".
+    iExists _; iFrame.
+    iPureIntro; etrans; done.
   Qed.
 
   Lemma sem_typed_seq Γ e1 e2 τ1 τ2 :
     Γ ⊨ e1 : τ1 -∗ Γ ⊨ e2 : τ2 -∗ Γ ⊨ Seq e1 e2 : τ2.
   Proof.
     iIntros "#IH1 #IH2" (Δ vs) "!# #HΓ"; simpl.
-    smart_wp_bind (SeqCtx _) v "#Hv" "IH1"; cbn.
+    iIntros (?) "?".
+    smart_wp_bind (SeqCtx _) v "Hv" "IH1"; cbn.
+    iDestruct "Hv" as (N1) "(#Hv&%&Hreg)".
     iApply wp_pure_step_later; auto 1 using to_of_val. iNext.
-    iApply "IH2"; done.
+    iApply (wp_wand with "[Hreg]"); first
+      iApply ("IH2" with "[] Hreg"); first done.
+    iIntros (w). iDestruct 1 as (N2) "(?&%&?)".
+    iExists _; iFrame.
+    iPureIntro; etrans; done.
   Qed.
 
   Lemma sem_typed_app Γ e1 e2 τ1 τ2 :
       Γ ⊨ e1 : TArrow τ1 τ2 -∗ Γ ⊨ e2 : τ1 -∗ Γ ⊨ App e1 e2 :  τ2.
   Proof.
     iIntros "#IH1 #IH2" (Δ vs) "!# #HΓ"; simpl.
-    smart_wp_bind (AppLCtx (e2.[env_subst vs])) v "#Hv" "IH1".
-    smart_wp_bind (AppRCtx v) w "#Hw" "IH2".
-    iApply "Hv"; done.
+    iIntros (?) "?".
+    smart_wp_bind (AppLCtx (e2.[env_subst vs])) v "Hv" "IH1".
+    iDestruct "Hv" as (N1) "(#Hv&%&Hreg)".
+    smart_wp_bind (AppRCtx v) w "Hw" "IH2".
+    iDestruct "Hw" as (N2) "(#Hw&%&Hreg)".
+    iApply (wp_wand with "[Hreg]"); first
+      iApply ("Hv" with "Hreg"); first done.
+    iIntros (w'). iDestruct 1 as (N3) "(?&%&?)".
+    iExists _; iFrame.
+    iPureIntro; etrans; first etrans; done.
   Qed.
 
   Lemma sem_typed_tlam Γ e τ :
     (subst (ren (+1)) <$> Γ) ⊨ e : τ -∗ Γ ⊨ TLam e : TForall τ.
   Proof.
     iIntros "#IH" (Δ vs) "!# #HΓ /=".
+    iIntros (?) "?".
     iApply wp_value; simpl.
-    iModIntro; iIntros (τi). iApply wp_pure_step_later; auto; iNext.
-    iApply "IH". by iApply interp_env_ren.
+    iExists _; iFrame; iSplit; last done.
+    iModIntro; iIntros (M' τi) "Hreg".
+    iApply wp_pure_step_later; auto; iNext.
+    iApply "IH"; last done. by iApply interp_env_ren.
   Qed.
 
   Lemma sem_typed_tapp Γ e τ τ' : Γ ⊨ e : TForall τ -∗ Γ ⊨ TApp e : τ.[τ'/].
   Proof.
     iIntros "#IH" (Δ vs) "!# #HΓ /=".
-    smart_wp_bind TAppCtx v "#Hv" "IH"; cbn.
+    iIntros (?) "?".
+    smart_wp_bind TAppCtx v "Hv" "IH"; cbn.
+    iDestruct "Hv" as (N1) "(#Hv&%&Hreg)".
     iApply wp_wand_r; iSplitL;
-      [iApply ("Hv" $! (⟦ τ' ⟧ Δ)); iPureIntro; apply _|]; cbn.
-    iIntros (w) "?". by iApply interp_subst.
+      first by iApply ("Hv" $! _ (⟦ τ' ⟧ Δ)).
+    iIntros (w). iDestruct 1 as (N3) "(?&%&?)".
+    iExists _; iFrame; iSplit; first by iApply interp_subst.
+    iPureIntro; etrans; done.
   Qed.
 
   Lemma sem_typed_pack Γ e τ τ' : Γ ⊨ e : τ.[τ'/] -∗ Γ ⊨ Pack e : TExist τ.
   Proof.
     iIntros "#IH" (Δ vs) "!##HΓ /=".
-    smart_wp_bind PackCtx v "#Hv" "IH". iApply wp_value.
+    iIntros (?) "?".
+    smart_wp_bind PackCtx v "Hv" "IH".
+    iDestruct "Hv" as (N1) "(#Hv&%&Hreg)".
+    iApply wp_value.
     rewrite -interp_subst.
-    iExists (interp _ Δ), _; iModIntro; iSplit; done.
+    iExists _; iFrame; iSplit; last done.
+    iModIntro. iExists (interp _ Δ), _; iSplit; done.
   Qed.
 
   Lemma sem_typed_unpack Γ e1 e2 τ τ' :
@@ -200,22 +296,29 @@ Section typed_interp.
     Γ ⊨ UnpackIn e1 e2 : τ'.
   Proof.
     iIntros "#IH1 #IH2" (Δ vs) "!# #HΓ /=".
-    smart_wp_bind (UnpackInCtx _) v "#Hv" "IH1".
+    iIntros (?) "?".
+    smart_wp_bind (UnpackInCtx _) v "Hv" "IH1".
+    iDestruct "Hv" as (N1) "(#Hv&%&Hreg)".
     iDestruct "Hv" as (τi w ->) "#Hw"; simpl.
     iApply wp_pure_step_later; auto 1 using to_of_val. iNext.
     asimpl.
     iApply wp_wand_r; iSplitL.
-    { iApply ("IH2" $! (τi :: Δ) (w :: vs) with "[]").
+    { iApply ("IH2" $! (τi :: Δ) (w :: vs) with "[] Hreg").
       iApply interp_env_cons; iSplit; first done.
       iApply interp_env_ren; done. }
-    iIntros (u) "Hu".
-    iApply (interp_weaken [] [_]); done.
+    iIntros (w'). iDestruct 1 as (N3) "(?&%&?)".
+    iExists _; iFrame; iSplit; first by iApply (interp_weaken [] [_]).
+    iPureIntro; etrans; done.
   Qed.
 
   Lemma sem_typed_fold Γ e τ : Γ ⊨ e : τ.[(TRec τ)/] -∗ Γ ⊨ Fold e : TRec τ.
   Proof.
     iIntros "#IH" (Δ vs) "!# #HΓ /=".
-    smart_wp_bind FoldCtx v "#Hv" ("IH" $! Δ vs). iApply wp_value.
+    iIntros (?) "?".
+    smart_wp_bind FoldCtx v "Hv" ("IH" $! Δ vs).
+    iDestruct "Hv" as (N1) "(#Hv&%&Hreg)".
+    iApply wp_value.
+    iExists _; iFrame; iSplit; last done.
     rewrite /= -interp_subst fixpoint_interp_rec1_eq /=.
     iModIntro; eauto.
   Qed.
@@ -223,28 +326,40 @@ Section typed_interp.
   Lemma sem_typed_unfold Γ e τ : Γ ⊨ e : TRec τ -∗ Γ ⊨ Unfold e : τ.[(TRec τ)/].
   Proof.
     iIntros "#IH" (Δ vs) "!# #HΓ /=".
-    smart_wp_bind UnfoldCtx v "#Hv" ("IH" $! Δ vs).
+    iIntros (?) "?".
+    smart_wp_bind UnfoldCtx v "Hv" ("IH" $! Δ vs).
+    iDestruct "Hv" as (N1) "(#Hv&%&Hreg)".
     rewrite /= fixpoint_interp_rec1_eq.
     change (fixpoint _) with (⟦ TRec τ ⟧ Δ); simpl.
     iDestruct "Hv" as (w) "#[% Hw]"; subst.
+    simpl.
     iApply wp_pure_step_later; cbn; auto using to_of_val.
-    iNext. iApply wp_value. by iApply interp_subst.
+    iNext. iApply wp_value.
+    iExists _; iFrame; iSplit; last done.
+    by iApply interp_subst.
   Qed.
 
   Lemma sem_typed_alloc Γ e τ : Γ ⊨ e : τ -∗ Γ ⊨ Alloc e : Tref τ.
   Proof.
     iIntros "#IH" (Δ vs) "!# #HΓ /=".
-    smart_wp_bind AllocCtx v "#Hv" "IH"; cbn. iClear "HΓ". iApply wp_fupd.
+    iIntros (?) "?".
+    smart_wp_bind AllocCtx v "Hv" "IH"; cbn.
+    iDestruct "Hv" as (N1) "(#Hv&%&Hreg)".
+    iClear "HΓ". iApply wp_fupd.
     iApply wp_alloc; auto 1 using to_of_val.
     iNext; iIntros (l) "Hl".
-    iMod (inv_alloc _ with "[Hl]") as "HN";
-      [| iModIntro; iExists _; iSplit; trivial]; eauto.
+    iMod (inv_alloc _ _ (∃ v : val, l ↦ᵢ v ∗ ⟦ τ ⟧ Δ v)%I with "[Hl]") as "HN".
+    { by iNext; iExists _; iFrame. }
+    iModIntro.
+    iExists _; iFrame; iSplit; [by eauto| done].
   Qed.
 
   Lemma sem_typed_load Γ e τ : Γ ⊨ e : (Tref τ) -∗ Γ ⊨ Load e : τ.
   Proof.
     iIntros "#IH" (Δ vs) "!# #HΓ /=".
-    smart_wp_bind LoadCtx v "#Hv" "IH"; cbn. iClear "HΓ".
+    iIntros (?) "?".
+    smart_wp_bind LoadCtx v "Hv" "IH"; cbn. iClear "HΓ".
+    iDestruct "Hv" as (N1) "(#Hv&%&Hreg)".
     iDestruct "Hv" as (l) "[% #Hv]"; subst.
     iApply wp_atomic.
     iInv (logN .@ l) as (w) "[Hw1 #Hw2]" "Hclose".
@@ -257,14 +372,20 @@ Section typed_interp.
     Γ ⊨ e1 : (Tref τ) -∗ Γ ⊨ e2 : τ -∗ Γ ⊨ Store e1 e2 : TUnit.
   Proof.
     iIntros "#IH1 #IH2" (Δ vs) "!# #HΓ /=".
-    smart_wp_bind (StoreLCtx _) v "#Hv" "IH1"; cbn.
-    smart_wp_bind (StoreRCtx _) w "#Hw" "IH2"; cbn. iClear "HΓ".
+    iIntros (?) "?".
+    smart_wp_bind (StoreLCtx _) v "Hv" "IH1"; cbn.
+    iDestruct "Hv" as (N1) "(#Hv&%&Hreg)".
+    smart_wp_bind (StoreRCtx _) w "Hw" "IH2"; cbn. iClear "HΓ".
+    iDestruct "Hw" as (N2) "(#Hw&%&Hreg)".
     iDestruct "Hv" as (l) "[% #Hv]"; subst.
     iApply wp_atomic.
     iInv (logN .@ l) as (z) "[Hz1 #Hz2]" "Hclose".
     iApply (wp_store with "Hz1"); auto using to_of_val.
     iModIntro. iNext.
-    iIntros "Hz1". iMod ("Hclose" with "[Hz1 Hz2]"); eauto.
+    iIntros "Hz1".
+    iMod ("Hclose" with "[Hz1 Hz2]") as "_"; first by eauto.
+    iModIntro; iExists _; iFrame; iSplit; first done.
+    iPureIntro; etrans; done.
   Qed.
 
   Theorem fundamental Γ e τ : Γ ⊢ₜ e : τ → ⊢ Γ ⊨ e : τ.
